rename stuff and separate into files

10_756_090.lean
@@ -1,215 +1,87 @@
-import TuringMachine2
+import TuringMachine.Defs
+import TuringMachine.Lemmas
 import Mathlib.Tactic.Linarith.Frontend
-import Mathlib.Data.Stream.Init
 
-inductive State where
-  | ST_A : State
-  | ST_B : State
-  | ST_C : State
-  | ST_D : State
-  | ST_E : State
+def transition : State5 -> Symbol2 -> Option State5 × Symbol2 × Direction
+  | State5.A, Symbol2.V0 => (some State5.B, Symbol2.V1, Direction.right)
+  | State5.A, Symbol2.V1 => (some State5.E, Symbol2.V1, Direction.right)
+  | State5.B, Symbol2.V0 => (some State5.C, Symbol2.V1, Direction.left )
+  | State5.B, Symbol2.V1 => (some State5.B, Symbol2.V1, Direction.right)
+  | State5.C, Symbol2.V0 => (some State5.A, Symbol2.V0, Direction.right)
+  | State5.C, Symbol2.V1 => (some State5.D, Symbol2.V0, Direction.left )
+  | State5.D, Symbol2.V0 => (some State5.B, Symbol2.V1, Direction.left )
+  | State5.D, Symbol2.V1 => (some State5.D, Symbol2.V1, Direction.left )
+  | State5.E, Symbol2.V0 => (none,          Symbol2.V1, Direction.left )
+  | State5.E, Symbol2.V1 => (some State5.A, Symbol2.V0, Direction.right)
 
-inductive Symbol where
-  | SYM_0 : Symbol
-  | SYM_1 : Symbol
+abbrev TM_10756090 := TuringMachine transition
 
-def Symbol.decEq (a b : Symbol) : Decidable (Eq a b) :=
-   match a, b with
-   | SYM_0, SYM_0 => isTrue rfl
-   | SYM_0, SYM_1  => isFalse (fun h => Symbol.noConfusion h)
-   | SYM_1, SYM_0  => isFalse (fun h => Symbol.noConfusion h)
-   | SYM_1, SYM_1   => isTrue rfl
-
-instance : DecidableEq Symbol :=
-   Symbol.decEq
-
-def transition : State -> Symbol -> Option State × Symbol × Direction :=
-  fun state symbol =>
-    match state, symbol with
-    | State.ST_A, Symbol.SYM_0 => (some State.ST_B, Symbol.SYM_1, Direction.right)
-    | State.ST_A, Symbol.SYM_1 => (some State.ST_E, Symbol.SYM_1, Direction.right)
-    | State.ST_B, Symbol.SYM_0 => (some State.ST_C, Symbol.SYM_1, Direction.left)
-    | State.ST_B, Symbol.SYM_1 => (some State.ST_B, Symbol.SYM_1, Direction.right)
-    | State.ST_C, Symbol.SYM_0 => (some State.ST_A, Symbol.SYM_0, Direction.right)
-    | State.ST_C, Symbol.SYM_1 => (some State.ST_D, Symbol.SYM_0, Direction.left)
-    | State.ST_D, Symbol.SYM_0 => (some State.ST_B, Symbol.SYM_1, Direction.left)
-    | State.ST_D, Symbol.SYM_1 => (some State.ST_D, Symbol.SYM_1, Direction.left)
-    | State.ST_E, Symbol.SYM_0 => (none,            Symbol.SYM_1, Direction.left)
-    | State.ST_E, Symbol.SYM_1 => (some State.ST_A, Symbol.SYM_0, Direction.right)
-
-def starting_machine : TuringMachine transition := 
-  TuringMachine.mk (Tape.blank Symbol.SYM_0) (State.ST_A)
+-- In state A and tape filled with zeroes 
+def starting_machine : TM_10756090 := 
+  TuringMachine.mk (Tape.blank Symbol2.V0) (State5.A)
 
 namespace proof
-
-def list_repeat {A : Type} (n : Nat) (x : List A) : List A :=
-  match n with
-  | 0 => []
-  | (n'+1) => x ++ list_repeat n' x
-
-def append_to_repeated {A : Type} (n : Nat) (l : List A) : Stream' A -> Stream' A :=
-  Stream'.appendStream' (list_repeat n l)
 
 -- state: C
 -- tape: C0 + n * [11] + [0] + n * [1]
 def A (n : Nat) : TuringMachine transition :=
-  let right_tape : Stream' Symbol := 
-    append_to_repeated (2*n) [Symbol.SYM_1] $
-    Stream'.cons Symbol.SYM_0 $
-    append_to_repeated n [Symbol.SYM_1] $
-    Stream'.const Symbol.SYM_0
-  let tape : Tape Symbol := Tape.mk (Stream'.const Symbol.SYM_0) Symbol.SYM_0 right_tape
-  TuringMachine.mk tape State.ST_C
+  let right_tape : Stream' Symbol2 := 
+    append_to_repeated (2*n) [Symbol2.V1] $
+    Stream'.cons Symbol2.V0 $
+    append_to_repeated n [Symbol2.V1] $
+    Stream'.const Symbol2.V0
+  let tape : Tape Symbol2 := Tape.mk (Stream'.const Symbol2.V0) Symbol2.V0 right_tape
+  TuringMachine.mk tape State5.C
 
 -- state: E
 -- tape: nl * [01] + E1 + nr * [11] + (nr + nl) * [1]
-def A' (nl : Nat) (nr : Nat) : TuringMachine transition :=
-  let left_tape : Stream' Symbol := 
-    append_to_repeated nl [Symbol.SYM_1, Symbol.SYM_0] $
-    Stream'.const Symbol.SYM_0
-  let right_tape : Stream' Symbol := 
-    append_to_repeated (2*nr) [Symbol.SYM_1] $
-    Stream'.cons Symbol.SYM_0 $
-    append_to_repeated (nr + nl) [Symbol.SYM_1] $
-    Stream'.const Symbol.SYM_0
-  TuringMachine.mk (Tape.mk left_tape Symbol.SYM_1 right_tape) State.ST_E
+def A' (nl : Nat) (nr : Nat) : TM_10756090 :=
+  let left_tape : Stream' Symbol2 := 
+    append_to_repeated nl [Symbol2.V1, Symbol2.V0] $
+    Stream'.const Symbol2.V0
+  let right_tape : Stream' Symbol2 := 
+    append_to_repeated (2*nr) [Symbol2.V1] $
+    Stream'.cons Symbol2.V0 $
+    append_to_repeated (nr + nl) [Symbol2.V1] $
+    Stream'.const Symbol2.V0
+  TuringMachine.mk (Tape.mk left_tape Symbol2.V1 right_tape) State5.E
 
 -- state: B
 -- tape: nl * [01] + nlm * [1] + D1 + nrm * [1] + [0] + nr * [1]
-def M (nl nlm nrm nr : Nat) : TuringMachine transition :=
-  let left_tape : Stream' Symbol := 
-    append_to_repeated nlm [Symbol.SYM_1] $
-    append_to_repeated nl [Symbol.SYM_1, Symbol.SYM_0] $
-    Stream'.const Symbol.SYM_0
-  let right_tape : Stream' Symbol := 
-    append_to_repeated nrm [Symbol.SYM_1] $
-    Stream'.cons Symbol.SYM_0 $
-    append_to_repeated nr [Symbol.SYM_1] $
-    Stream'.const Symbol.SYM_0
-  TuringMachine.mk (Tape.mk left_tape Symbol.SYM_1 right_tape) State.ST_B
+def M (nl nlm nrm nr : Nat) : TM_10756090 :=
+  let left_tape : Stream' Symbol2 := 
+    append_to_repeated nlm [Symbol2.V1] $
+    append_to_repeated nl [Symbol2.V1, Symbol2.V0] $
+    Stream'.const Symbol2.V0
+  let right_tape : Stream' Symbol2 := 
+    append_to_repeated nrm [Symbol2.V1] $
+    Stream'.cons Symbol2.V0 $
+    append_to_repeated nr [Symbol2.V1] $
+    Stream'.const Symbol2.V0
+  TuringMachine.mk (Tape.mk left_tape Symbol2.V1 right_tape) State5.B
 
 -- state: D
 -- tape: nl * [01] + nlm * [1] + D1 + nrm * [1] + [0] + nr * [1]
-def M' (nl nlm nrm nr : Nat) : TuringMachine transition :=
-  let left_tape : Stream' Symbol := 
-    append_to_repeated nlm [Symbol.SYM_1] $
-    append_to_repeated nl [Symbol.SYM_1, Symbol.SYM_0] $
-    Stream'.const Symbol.SYM_0
-  let right_tape : Stream' Symbol := 
-    append_to_repeated nrm [Symbol.SYM_1] $
-    Stream'.cons Symbol.SYM_0 $
-    append_to_repeated nr [Symbol.SYM_1] $
-    Stream'.const Symbol.SYM_0
-  TuringMachine.mk (Tape.mk left_tape Symbol.SYM_1 right_tape) State.ST_D
+def M' (nl nlm nrm nr : Nat) : TM_10756090 :=
+  let left_tape : Stream' Symbol2 := 
+    append_to_repeated nlm [Symbol2.V1] $
+    append_to_repeated nl [Symbol2.V1, Symbol2.V0] $
+    Stream'.const Symbol2.V0
+  let right_tape : Stream' Symbol2 := 
+    append_to_repeated nrm [Symbol2.V1] $
+    Stream'.cons Symbol2.V0 $
+    append_to_repeated nr [Symbol2.V1] $
+    Stream'.const Symbol2.V0
+  TuringMachine.mk (Tape.mk left_tape Symbol2.V1 right_tape) State5.D
 
-theorem reaches_A1 : TuringMachine.advance^[5] starting_machine = A 1 := rfl
-
-theorem append_one_eq_cons (s : Symbol) : append_to_repeated 1 [s] = Stream'.cons s := rfl
-
-theorem append_two_eq_cons (s1 s2 : Symbol) : append_to_repeated 1 [s1, s2] = Stream'.cons s1 ∘ Stream'.cons s2 := rfl
-
-theorem append_sum : append_to_repeated (n + k) l s = (append_to_repeated n l $ append_to_repeated k l s) := by
-  induction n with
-  | zero =>
-    rw [Nat.zero_add]
-    rfl
-  | succ n' ih =>
-    rw [←Nat.add_one, Nat.add_assoc]
-    simp [Nat.add_comm]
-    rw [←Nat.add_assoc]
-    unfold append_to_repeated
-    conv =>
-      pattern list_repeat (n' + 1) l 
-      unfold list_repeat
-    conv => lhs; unfold list_repeat
-    simp
-    unfold append_to_repeated at ih
-    rw [Stream'.append_append_stream]
-    conv => rhs; rw [Stream'.append_append_stream]
-    rw [ih]
-
-theorem append_get' (h : k < n) : (append_to_repeated n [a] s) k = a := by
-  induction n with
-  | zero =>
-    exact False.elim $ Nat.not_lt_zero k h
-  | succ n' =>
-    unfold append_to_repeated
-    unfold list_repeat
-    cases k with
-    | zero => rfl
-    | succ k' => 
-      rw [Stream'.append_append_stream]
-      unfold Stream'.appendStream'
-      unfold Stream'.cons
-      simp
-      rw [Stream'.nil_append_stream]
-      have h' : k' < n' := by rw [←Nat.add_one, ←Nat.add_one] at h; exact Nat.lt_of_add_lt_add_right h
-      exact append_get' h'
-
-theorem get_drop (n m : Nat) (s : Stream' α) : (Stream'.drop m s) n = s (n + m) :=
-  rfl
-
-theorem append_get (k n : Nat) (l : List T) (s : Stream' T) : (append_to_repeated k l s) (l.length * k + n) = s n := by
-  cases k with
-  | zero =>
-    simp
-    rfl
-  | succ k' => 
-    rw [←Nat.add_one, append_sum, Nat.left_distrib, Nat.add_assoc]
-    rw [append_get k' (l.length * 1 + n) l (append_to_repeated 1 l s)]
-    unfold append_to_repeated
-    unfold list_repeat
-    unfold list_repeat
-    simp
-    rw [Nat.add_comm]
-    rw [←get_drop n l.length (l ++ₛ s)]
-    rw [Stream'.drop_append_stream]
-
-theorem append_stream_one {A : Type} (x : A) (xs : List A) :
-  Stream'.appendStream' (x :: xs) = Stream'.cons x ∘ Stream'.appendStream' xs
-  := rfl
-
-theorem list_repeat_one_cons {A : Type} (n : Nat) (s : A) :
-  list_repeat (n + 1) [s] = s :: list_repeat n [s]
-  := rfl
-
-theorem append_repeated_zero (l : List Symbol) :
-  append_to_repeated 0 l = id := rfl
-
-theorem append_repeated_one (n : Nat) (s : Symbol) :
-  append_to_repeated (n + 1) [s] = append_to_repeated 1 [s] ∘ append_to_repeated n [s]
-  := by
-    rw [append_one_eq_cons]
-    have : append_to_repeated (n + 1) [s] = Stream'.appendStream' (list_repeat (n + 1) [s]) := rfl
-    rw [this, list_repeat_one_cons, append_stream_one]
-    rfl
-
-theorem cons_to_const (s : Symbol) : Stream'.cons s (Stream'.const s) = (Stream'.const s) := by
-  funext n
-  cases n <;> rfl
-
-def tm_succeeds {Q Γ : Type _} {δ : Q -> Γ -> (Option Q × Γ × Direction)} (tm1 tm2 : TuringMachine δ) :=
-  ∃n : Nat, (TuringMachine.advance^[n] tm1) = tm2
-
-infix:60 " =>> " => tm_succeeds
-
-theorem trans_succeeds {tm1 tm2 tm3 : TuringMachine δ} (h1 : tm1 =>> tm2) (h2 : tm2 =>> tm3) : tm1 =>> tm3 := by
-  let ⟨n1, t1⟩ := h1
-  let ⟨n2, t2⟩ := h2
-  exists (n2 + n1)
-  rw [Function.iterate_add_apply, t1, t2]
-
-instance : Trans (tm_succeeds (Q := Q) (Γ := Γ) (δ := δ)) tm_succeeds tm_succeeds where
-  trans := trans_succeeds
-
-theorem A'_to_M_ : A' (n + 1) 0 =>> M (n + 2) 0 n 0 := by
+lemma A'_to_M : A' (n + 1) 0 =>> M (n + 2) 0 n 0 := by
   unfold tm_succeeds
   exists 2
   ext : 1
   . ext : 1
     repeat rfl
     . have t1 : (TuringMachine.advance^[2] (A' (n + 1) 0)).tape.right_half = 
-        (append_to_repeated n [Symbol.SYM_1] $ Stream'.const Symbol.SYM_0) := by
+        (append_to_repeated n [Symbol2.V1] $ Stream'.const Symbol2.V0) := by
           conv => arg 2; rw [←Nat.zero_add n]
       unfold M; conv => rhs; simp
       rw [append_repeated_zero, t1]
@@ -217,44 +89,44 @@ theorem A'_to_M_ : A' (n + 1) 0 =>> M (n + 2) 0 n 0 := by
       rw [cons_to_const]
   . rfl
 
-theorem M_to_M_iter_ : M nl nlm nrm nr =>> M nl (nlm + nrm) 0 nr := by
+lemma M_to_M_iter : M nl nlm nrm nr =>> M nl (nlm + nrm) 0 nr := by
   cases nrm
   . exists 0
   case succ nrm' =>
     calc M nl nlm (nrm' + 1) nr
       _ =>> M nl (nlm + 1) nrm' nr       := by exists 1
-      _ =>> M nl (nlm + 1 + nrm') 0 nr   := M_to_M_iter_
+      _ =>> M nl (nlm + 1 + nrm') 0 nr   := M_to_M_iter
       _ =   M nl (nlm + (nrm' + 1)) 0 nr := by rw [Nat.add_assoc]; conv => lhs; arg 2; arg 2; rw [Nat.add_comm]
 
-theorem M'_to_M'_iter_ : M' nl nlm nrm nr =>> M' nl 0 (nrm + nlm) nr := by
+lemma M'_to_M'_iter : M' nl nlm nrm nr =>> M' nl 0 (nrm + nlm) nr := by
   cases nlm
   . exists 0
   case succ nlm' =>
     calc M' nl (nlm' + 1) nrm nr
       _ =>> M' nl nlm' (nrm + 1) nr       := by exists 1
-      _ =>> M' nl 0 (nrm + 1 + nlm') nr   := M'_to_M'_iter_
+      _ =>> M' nl 0 (nrm + 1 + nlm') nr   := M'_to_M'_iter
       _ =   M' nl 0 (nrm + (nlm' + 1)) nr := by
         rw [Nat.add_assoc]
         conv => lhs; arg 3; arg 2; rw [Nat.add_comm]
 
-theorem Ml_to_M'l_ : M nl 0 (nm + 1) nr =>> M' nl 0 nm (nr + 1) := by
+lemma Ml_to_M' : M nl 0 (nm + 1) nr =>> M' nl 0 nm (nr + 1) := by
   calc M nl 0 (nm + 1) nr
-    _ =>> M nl (0 + (nm + 1)) 0 nr  := M_to_M_iter_
+    _ =>> M nl (0 + (nm + 1)) 0 nr  := M_to_M_iter
     _ =   M nl (nm + 1) 0 nr        := by simp
     _ =>> M' nl nm 0 (nr + 1)       := by exists 3
-    _ =>> M' nl 0 (0 + nm) (nr + 1) := M'_to_M'_iter_
+    _ =>> M' nl 0 (0 + nm) (nr + 1) := M'_to_M'_iter
     _ =   M' nl 0 nm (nr + 1)       := by rw [Nat.zero_add]
 
-theorem Ml_to_Ml_ : M (nl + 2) 0 (nm + 1) nr =>> M (nl + 1) 0 (nm + 2) (nr + 1) := by
+lemma Ml_to_Ml : M (nl + 2) 0 (nm + 1) nr =>> M (nl + 1) 0 (nm + 2) (nr + 1) := by
   calc M (nl + 2) 0 (nm + 1) nr
-    _ =>> M' (nl + 2) 0 nm (nr + 1)      := Ml_to_M'l_
+    _ =>> M' (nl + 2) 0 nm (nr + 1)      := Ml_to_M'
     _ =>> M (nl + 1) 0 (nm + 2) (nr + 1) := by exists 4
 
-theorem Ml_to_A_iter : M (nl + 1) 0 (2 * nr + nl + 1) (nr + 1) =>> A (nl + nr + 2) := by
+lemma Ml_to_A_iter : M (nl + 1) 0 (2 * nr + nl + 1) (nr + 1) =>> A (nl + nr + 2) := by
   cases nl
   . simp
     calc M 1 0 (2 * nr + 1) (nr + 1)
-      _ =>> M' 1 0 (2 * nr) (nr + 2) := Ml_to_M'l_
+      _ =>> M' 1 0 (2 * nr) (nr + 2) := Ml_to_M'
       _ =>> A (nr + 2)               := by exists 4
   case succ nl' =>
     have t1 : 2 * nr + (nl' + 1) + 1 = 2 * nr + 1 + nl' + 1 := by linarith
@@ -262,12 +134,12 @@ theorem Ml_to_A_iter : M (nl + 1) 0 (2 * nr + nl + 1) (nr + 1) =>> A (nl + nr + 
     have t3 : (nl' + 1) + nr + 2 = nl' + (nr + 1) + 2       := by linarith
     calc M (nl' + 2) 0 (2 * nr + (nl' + 1) + 1) (nr + 1)
       _ =   M (nl' + 2) 0 ((2*nr + 1 + nl') + 1) (nr + 1)   := by rw [t1]
-      _ =>> M (nl' + 1) 0 ((2*nr + 1 + nl') + 2) (nr + 2)   := Ml_to_Ml_
+      _ =>> M (nl' + 1) 0 ((2*nr + 1 + nl') + 2) (nr + 2)   := Ml_to_Ml
       _ =   M (nl' + 1) 0 (2 * (nr + 1) + nl' + 1) (nr + 2) := by rw [t2]
       _ =>> A (nl' + (nr + 1) + 2) := Ml_to_A_iter
       _ =   A ((nl' + 1) + nr + 2) := by rw [t3]
 
-theorem A'_to_A'_ : A' nl (nr + 1) =>> A' (nl + 1) nr := by
+lemma A'_to_A' : A' nl (nr + 1) =>> A' (nl + 1) nr := by
   exists 2
   ext : 1
   . ext : 1
@@ -279,89 +151,49 @@ theorem A'_to_A'_ : A' nl (nr + 1) =>> A' (nl + 1) nr := by
       rfl
   . rfl
 
-theorem A'_to_A'_iter_ : A' nl nr =>> A' (nl + nr) 0 := by
+lemma A'_to_A'_iter : A' nl nr =>> A' (nl + nr) 0 := by
   cases nr
   . exists 0
   case succ nr' =>
     have t1 : nl + 1 + nr' = nl + (nr' + 1) := by linarith
     calc A' nl (nr' + 1)
-      _ =>> A' (nl + 1) nr'       := A'_to_A'_
-      _ =>> A' (nl + 1 + nr') 0   := A'_to_A'_iter_
+      _ =>> A' (nl + 1) nr'       := A'_to_A'
+      _ =>> A' (nl + 1 + nr') 0   := A'_to_A'_iter
       _ =   A' (nl + (nr' + 1)) 0 := by rw [t1]
 
-theorem A_to_A_ : A (n + 2) =>> A (n + 3) := by
+theorem A_to_A : A (n + 2) =>> A (n + 3) := by
   calc A (n + 2)
     _ =>> A' 1 (n + 1)          := by exists 2
-    _ =>> A' (1 + (n + 1)) 0    := A'_to_A'_iter_
+    _ =>> A' (1 + (n + 1)) 0    := A'_to_A'_iter
     _ =   A' (n + 2) 0          := by rw [Nat.add_comm]
-    _ =>> M (n + 3) 0 (n + 1) 0 := A'_to_M_
-    _ =>> M (n + 2) 0 (n + 2) 1 := Ml_to_Ml_
+    _ =>> M (n + 3) 0 (n + 1) 0 := A'_to_M
+    _ =>> M (n + 2) 0 (n + 2) 1 := Ml_to_Ml
     _ =   M (n + 2) 0 (2 * 0 + (n + 1) + 1) 1 := by simp
     _ =>> A (n + 3) := Ml_to_A_iter
 
-theorem halted_to_halted (tm : TuringMachine transition) (k : Nat) (h : ¬(TuringMachine.is_not_halted tm)) : ¬(TuringMachine.is_not_halted (TuringMachine.advance^[k] tm)) :=
-  match k with
-  | 0 => h
-  | k' + 1 => by
-    simp [Function.iterate_add_apply]
-    apply halted_to_halted (TuringMachine.advance tm) k'
-    let (TuringMachine.mk tape state) := tm
-    cases state
-    . let tm' : TuringMachine transition := TuringMachine.advance { tape := tape, state := none }
-      have : tm'.state = none := rfl
-      let (TuringMachine.mk tape' state') := tm'
-      cases state'
-      . intro hnh
-        exact (Bool.self_ne_not false) hnh  
-      . contradiction
-    . contradiction
-
-theorem not_halted_if_next_not_halted (tm : TuringMachine transition) (h : (TuringMachine.advance tm).is_not_halted) : tm.is_not_halted := by
-  unfold TuringMachine.is_not_halted
-  rw [←Option.ne_none_iff_isSome]
-  intro hn
-  have : tm.advance.state = none := by
-    unfold TuringMachine.advance
-    simp [hn]
-  unfold TuringMachine.advance at h
-  simp [hn] at h
-  unfold TuringMachine.is_not_halted at h
-  rw [hn] at h
-  simp at h
-
-theorem not_halted_if_later_not_halted (tm : TuringMachine transition) (k : Nat) (h : TuringMachine.is_not_halted (TuringMachine.advance^[k] tm)) : TuringMachine.is_not_halted tm := by
-  induction k with
-  | zero => exact h
-  | succ k' ih =>
-    have := not_halted_if_next_not_halted (TuringMachine.advance^[k'] tm)
-    conv at this => arg 1; arg 1; rw [←Function.iterate_one TuringMachine.advance]; arg 3; simp
-    rw [←Function.iterate_add_apply] at this
-    rw [Nat.add_comm] at this
-    exact ih (this h)
-
-theorem A_to_any_A_ (k : Nat) : ∃m : Nat, (TuringMachine.advance^[m] (A 2)) = A (k + 2) ∧ k <= m := by
+lemma A_to_any_A (k : Nat) : ∃m : Nat, (TuringMachine.advance^[m] (A 2)) = A (k + 2) ∧ k <= m := by
   induction k with
   | zero => exists 0
   | succ k' ih =>
     let ⟨m', ⟨h1, h2⟩⟩ := ih
-    let ⟨m'', hm⟩ : A (k' + 2) =>> A (k' + 3) := A_to_A_
+    let ⟨m'', hm⟩ : A (k' + 2) =>> A (k' + 3) := A_to_A
     have t1 : 1 <= m'' := by
       have t2 : A (k' + 2) ≠ A (k' + 3) := by
-        have t4 : (A (k' + 2)).tape.right_half (2 * (k' + 2)) = Symbol.SYM_0 := by
+        have t4 : (A (k' + 2)).tape.right_half (2 * (k' + 2)) = Symbol2.V0 := by
           unfold A; simp
-          have t3 := append_get (2 * (k' + 2)) 0 [Symbol.SYM_1]
+          have t3 := append_get (2 * (k' + 2)) 0 [Symbol2.V1]
           simp at t3
           rw [t3]
           rfl
-        have t5 : (A (k' + 3)).tape.right_half (2 * (k' + 2)) = Symbol.SYM_1 := by
+        have t5 : (A (k' + 3)).tape.right_half (2 * (k' + 2)) = Symbol2.V1 := by
           unfold A; simp
           have : 2 * (k' + 2) < 2 * (k' + 3) := by simp
-          rw [append_get' (a := Symbol.SYM_1) this]
+          rw [append_get' (a := Symbol2.V1) this]
         intro h
         have := congr_arg (fun x => x.tape.right_half (1 * (2 * (k' + 2)))) h
         simp at this
         rw [t4, t5] at this
-        have t7 : Symbol.SYM_0 ≠ Symbol.SYM_1 := by decide
+        have t7 : Symbol2.V0 ≠ Symbol2.V1 := by decide
         exact t7 this
       rw [Nat.one_le_iff_ne_zero]
       intro hm''z
@@ -373,9 +205,9 @@ theorem A_to_any_A_ (k : Nat) : ∃m : Nat, (TuringMachine.advance^[m] (A 2)) = 
     . rw [Nat.add_comm]
       exact Nat.add_le_add h2 t1 
 
-theorem reaches_A2 : TuringMachine.advance^[23] starting_machine = A 2 := rfl
+lemma reaches_A2 : TuringMachine.advance^[23] starting_machine = A 2 := rfl
 
-theorem any_to_A (n : Nat) : ∃ m k : Nat, TuringMachine.advance^[n + k] starting_machine = A (m + 2) :=
+lemma any_to_A (n : Nat) : ∃ m k : Nat, TuringMachine.advance^[n + k] starting_machine = A (m + 2) :=
   Decidable.casesOn (Nat.decLe n 23)
     (fun t => by
       rw [Nat.not_le] at t
@@ -383,7 +215,7 @@ theorem any_to_A (n : Nat) : ∃ m k : Nat, TuringMachine.advance^[n + k] starti
       let ⟨n', hn'⟩ := Nat.exists_eq_add_of_le this
       rw [hn']
       exists (n' + 1)
-      have ⟨m', ⟨hm', hm''⟩⟩ := A_to_any_A_ (n' + 1)
+      have ⟨m', ⟨hm', hm''⟩⟩ := A_to_any_A (n' + 1)
       rw [←reaches_A2] at hm'
       rw [←Function.iterate_add_apply] at hm'
       exists (m' - n' - 1)
