Main.lean
@@ -1,8 +1,7 @@
 import Mathlib.Data.Vector
 import Mathlib.Data.Nat.Order.Basic
 
--- import TuringMachine
-import TuringMachine2
+import TuringMachine.Defs
 -- import 10_756_090
 
 def main (args : List String) : IO Unit := IO.println args.head!
@@ -11,28 +10,28 @@ lemma vec_mul_take {α : Type _} (x : Nat) (y : Nat) : Vector α (min x (x * (y 
   rw [Nat.min_eq_left $ Nat.le_mul_of_pos_right $ Nat.succ_pos y]
 
 lemma vec_mul_drop {α : Type _} (x : Nat) (y : Nat) : Vector α (x * (y + 1) - x) = Vector α (x * y) := by
-  have t1 : x * (y + 1) = x * y + x := rfl;
+  have t1 : x * (y + 1) = x * y + x := rfl
   simp [t1]
 
 lemma vec_tail_len {α : Type _} {n : Nat} {a : α} {as : List α} (h : List.length (a :: as) = n+1) : List.length as = n := by
-  have tc : List.tail (a :: as) = as := List.tail_cons;
+  have tc : List.tail (a :: as) = as := List.tail_cons
   rw [←tc, List.length_tail]
   exact congr_arg Nat.pred h
 
 def vec_chunks {α : Type _} : (x : Nat) → (y : Nat) → (v : Vector α (x * y)) → Vector (Vector α x) y
   | _, 0, _ => Vector.nil
   | x, y'+1, v =>
-    let v'   : Vector α (x * y') := cast (vec_mul_drop x y') (v.drop x);
-    let head : Vector α x        := cast (vec_mul_take x y') (v.take x);
+    let v'   : Vector α (x * y') := cast (vec_mul_drop x y') (v.drop x)
+    let head : Vector α x        := cast (vec_mul_take x y') (v.take x)
     Vector.cons head $ vec_chunks x y' v'
 
 def vec_mapM {α : Type _} {β : Type _} {n : Nat} (f : α → Option β) (as : Vector α n) : Option (Vector β n) :=
   match n with
   | 0 => some Vector.nil
   | n'+1 =>
-    let ⟨a' :: as', h⟩ := as;
-    let b : Option β := f a';
-    let bs : Option (Vector β n') := vec_mapM f ⟨as', vec_tail_len h⟩;
+    let ⟨a' :: as', h⟩ := as
+    let b : Option β := f a'
+    let bs : Option (Vector β n') := vec_mapM f ⟨as', vec_tail_len h⟩
     match b, bs with
     | some b', some bs' => some (Vector.cons b' bs')
     | _, _ => none
@@ -60,7 +59,7 @@ def parse_direction : (c : Char) → Option Direction
   | _ => none
 
 def parse_transition (n : Nat) (m : Nat) (chars : Vector Char 3) : Option $ Option (Fin n × Fin m × Direction) :=
-  let ⟨sym :: dir :: state :: [], _⟩ := chars;
+  let ⟨sym :: dir :: state :: [], _⟩ := chars
   if let ('-', '-', '-') := (sym, dir, state) then
     some none
   else if let (some sym', some state', some dir') := (parse_symbol n sym, parse_state m sym, parse_direction dir) then
@@ -73,19 +72,19 @@ def parse_transition (n : Nat) (m : Nat) (chars : Vector Char 3) : Option $ Opti
     none
 
 def parse_state_transitions (n : Nat) (m : Nat) (chars : Vector Char (3 * m + 1)) : Option (Vector (Option (Fin n × Fin m × Direction)) m) :=
-  let ⟨_ :: cs, h⟩ := chars;
-  let transitions := vec_chunks 3 m ⟨cs, vec_tail_len h⟩;
+  let ⟨_ :: cs, h⟩ := chars
+  let transitions := vec_chunks 3 m ⟨cs, vec_tail_len h⟩
   vec_mapM (parse_transition n m) transitions
 
 -- Fails if n or m is too large
 def parse_transition_table : (n : Nat) → (m : Nat) → String → Option (Vector (Vector (Option (Fin n × Fin m × Direction)) m) n)
   | n, m, s =>
-    let input : List Char := '_' :: s.data;
+    let input : List Char := '_' :: s.data
     Decidable.casesOn (decEq input.length ((3 * m + 1) * n))
       (fun _ => none)
       (
         fun h =>
-          let states := vec_chunks (3 * m + 1) n ⟨input, h⟩;
+          let states := vec_chunks (3 * m + 1) n ⟨input, h⟩
           vec_mapM (parse_state_transitions n m) states
       )
 
