TuringMachine/Lemmas.lean
@@ -1,0 +1,176 @@
+import Mathlib.Data.Stream.Defs
+import Mathlib.Logic.Function.Iterate
+import Mathlib.Data.Stream.Init
+import TuringMachine.Defs
+
+variable {Q Γ : Type _}
+variable {δ : Q -> Γ -> Option Q × Γ × Direction}
+
+
+inductive State5 where
+  | A : State5
+  | B : State5
+  | C : State5
+  | D : State5
+  | E : State5
+
+inductive Symbol2 where
+  | V0 : Symbol2
+  | V1 : Symbol2
+
+def Symbol2.decEq (a b : Symbol2) : Decidable (Eq a b) :=
+   match a, b with
+   | V0, V0 => isTrue rfl
+   | V0, V1  => isFalse (fun h => Symbol2.noConfusion h)
+   | V1, V0  => isFalse (fun h => Symbol2.noConfusion h)
+   | V1, V1   => isTrue rfl
+
+instance : DecidableEq Symbol2 :=
+   Symbol2.decEq
+
+def list_repeat (n : Nat) (x : List Γ) : List Γ :=
+  match n with
+  | 0 => []
+  | (n'+1) => x ++ list_repeat n' x
+
+def append_to_repeated (n : Nat) (l : List Γ) : Stream' Γ -> Stream' Γ :=
+  Stream'.appendStream' (list_repeat n l)
+
+theorem append_one_eq_cons (s : Γ) : append_to_repeated 1 [s] = Stream'.cons s := rfl
+
+theorem append_two_eq_cons (s1 s2 : Γ) : append_to_repeated 1 [s1, s2] = Stream'.cons s1 ∘ Stream'.cons s2 := rfl
+
+theorem append_sum : append_to_repeated (n + k) l s = (append_to_repeated n l $ append_to_repeated k l s) := by
+  induction n with
+  | zero =>
+    rw [Nat.zero_add]
+    rfl
+  | succ n' ih =>
+    rw [←Nat.add_one, Nat.add_assoc]
+    simp [Nat.add_comm]
+    rw [←Nat.add_assoc]
+    unfold append_to_repeated
+    conv =>
+      pattern list_repeat (n' + 1) l 
+      unfold list_repeat
+    conv => lhs; unfold list_repeat
+    simp
+    unfold append_to_repeated at ih
+    rw [Stream'.append_append_stream]
+    conv => rhs; rw [Stream'.append_append_stream]
+    rw [ih]
+
+theorem append_get' (h : k < n) : (append_to_repeated n [a] s) k = a := by
+  induction n with
+  | zero =>
+    exact False.elim $ Nat.not_lt_zero k h
+  | succ n' =>
+    unfold append_to_repeated
+    unfold list_repeat
+    cases k with
+    | zero => rfl
+    | succ k' => 
+      rw [Stream'.append_append_stream]
+      unfold Stream'.appendStream'
+      unfold Stream'.cons
+      simp
+      rw [Stream'.nil_append_stream]
+      have h' : k' < n' := by rw [←Nat.add_one, ←Nat.add_one] at h; exact Nat.lt_of_add_lt_add_right h
+      exact append_get' h'
+
+theorem get_drop (n m : Nat) (s : Stream' α) : (Stream'.drop m s) n = s (n + m) :=
+  rfl
+
+theorem append_get (k n : Nat) (l : List T) (s : Stream' T) : (append_to_repeated k l s) (l.length * k + n) = s n := by
+  cases k with
+  | zero =>
+    simp
+    rfl
+  | succ k' => 
+    rw [←Nat.add_one, append_sum, Nat.left_distrib, Nat.add_assoc]
+    rw [append_get k' (l.length * 1 + n) l (append_to_repeated 1 l s)]
+    unfold append_to_repeated
+    unfold list_repeat
+    unfold list_repeat
+    simp
+    rw [Nat.add_comm]
+    rw [←get_drop n l.length (l ++ₛ s)]
+    rw [Stream'.drop_append_stream]
+
+theorem append_stream_one (x : Γ) (xs : List Γ) :
+  Stream'.appendStream' (x :: xs) = Stream'.cons x ∘ Stream'.appendStream' xs
+    := rfl
+
+theorem list_repeat_one_cons (n : Nat) (s : Γ) :
+  list_repeat (n + 1) [s] = s :: list_repeat n [s]
+    := rfl
+
+theorem append_repeated_zero (l : List Γ) :
+  append_to_repeated 0 l = id := rfl
+
+theorem append_repeated_one (n : Nat) (s : Γ) :
+  append_to_repeated (n + 1) [s] = append_to_repeated 1 [s] ∘ append_to_repeated n [s]
+  := by
+    rw [append_one_eq_cons]
+    have : append_to_repeated (n + 1) [s] = Stream'.appendStream' (list_repeat (n + 1) [s]) := rfl
+    rw [this, list_repeat_one_cons, append_stream_one]
+    rfl
+
+theorem cons_to_const (s : Γ) : Stream'.cons s (Stream'.const s) = (Stream'.const s) := by
+  funext n
+  cases n <;> rfl
+
+def tm_succeeds (tm1 tm2 : TuringMachine δ) :=
+  ∃n : Nat, (TuringMachine.advance^[n] tm1) = tm2
+
+infix:60 " =>> " => tm_succeeds
+
+theorem trans_succeeds {tm1 tm2 tm3 : TuringMachine δ} (h1 : tm1 =>> tm2) (h2 : tm2 =>> tm3) : tm1 =>> tm3 := by
+  let ⟨n1, t1⟩ := h1
+  let ⟨n2, t2⟩ := h2
+  exists (n2 + n1)
+  rw [Function.iterate_add_apply, t1, t2]
+
+instance : Trans (tm_succeeds (Q := Q) (Γ := Γ) (δ := δ)) tm_succeeds tm_succeeds where
+  trans := trans_succeeds
+
+theorem halted_to_halted (tm : TuringMachine δ) (k : Nat) (h : ¬(TuringMachine.is_not_halted tm)) : ¬(TuringMachine.is_not_halted (TuringMachine.advance^[k] tm)) :=
+  match k with
+  | 0 => h
+  | k' + 1 => by
+    simp [Function.iterate_add_apply]
+    apply halted_to_halted (TuringMachine.advance tm) k'
+    let (TuringMachine.mk tape state) := tm
+    cases state
+    . let tm' : TuringMachine δ := TuringMachine.advance { tape := tape, state := none }
+      have : tm'.state = none := rfl
+      let (TuringMachine.mk tape' state') := tm'
+      cases state'
+      . intro hnh
+        exact (Bool.self_ne_not false) hnh  
+      . contradiction
+    . contradiction
+
+theorem not_halted_if_next_not_halted (tm : TuringMachine δ) (h : (TuringMachine.advance tm).is_not_halted) : tm.is_not_halted := by
+  unfold TuringMachine.is_not_halted
+  rw [←Option.ne_none_iff_isSome]
+  intro hn
+  have : tm.advance.state = none := by
+    unfold TuringMachine.advance
+    simp [hn]
+  unfold TuringMachine.advance at h
+  simp [hn] at h
+  unfold TuringMachine.is_not_halted at h
+  rw [hn] at h
+  simp at h
+
+theorem not_halted_if_later_not_halted (tm : TuringMachine δ) (k : Nat) (h : TuringMachine.is_not_halted (TuringMachine.advance^[k] tm)) : TuringMachine.is_not_halted tm := by
+  induction k with
+  | zero => exact h
+  | succ k' ih =>
+    have := not_halted_if_next_not_halted (TuringMachine.advance^[k'] tm)
+    conv at this => arg 1; arg 1; rw [←Function.iterate_one TuringMachine.advance]; arg 3; simp
+    rw [←Function.iterate_add_apply] at this
+    rw [Nat.add_comm] at this
+    exact ih (this h)
+
